examples/refinement/sum_and_swap.fst
@@ -21,15 +21,21 @@ let swap_and_sum () =
 
 // WP for sum and swap
 unfold
-let sum_wp : hwp int  = fun s0 post -> let (r1, r2) = s0 in post (U32.v r1 + U32.v r2, (r2, r1))
+let sum_wp : (wp:hwp int{monotonic wp}) = 
+  let wp = 
+    fun s0 post -> let (r1, r2) = s0 in post (U32.v r1 + U32.v r2, (r2, r1))
+  in
+  assume (monotonic wp);
+  wp
+
 
 // Hardwritten for now but can be easily computed with a tactic (if there isn't support for this already)
 unfold 
-let sum_wp_full : hwp int = 
-  bind_wp mint int (read_wp 0) (fun x0 ->
-  bind_wp mint int (read_wp 1) (fun x1 ->
-  bind_wp unit int (write_wp 0 x1) (fun () ->
-  bind_wp unit int (write_wp 1 x0) (fun () ->
+let sum_wp_full : (wp:hwp int{monotonic wp}) = 
+  bind_wp (read_wp 0) (fun x0 ->
+  bind_wp (read_wp 1) (fun x1 ->
+  bind_wp (write_wp 0 x1) (fun () ->
+  bind_wp (write_wp 1 x0) (fun () ->
   return_wp (U32.v x0 + U32.v x1)))))
 
 
@@ -44,7 +50,7 @@ let sum_post = fun s0 res -> let (x, s1) = res in
                           x = U32.v r1 + U32.v r2 /\
                           r1 = r2' /\ r2 = r1'
 
-val hswap_and_sum : unit -> HIGH int sum_wp 
+val hswap_and_sum : unit -> HIGH int sum_wp_full 
 let hswap_and_sum () = 
   let x0 = HIGH?.get 0 in 
   let x1 = HIGH?.get 1 in 
@@ -52,7 +58,7 @@ let hswap_and_sum () =
   let _  = HIGH?.put 1 x0 in
   U32.v x0 + U32.v x1
 
-val swap_and_sum' : unit -> comp_wp' int sum_wp 
+val swap_and_sum' : unit -> comp_wp int sum_wp_full
 let swap_and_sum' () =  
   bind_elab (hread' 0) (fun x0 -> 
   bind_elab (hread' 1) (fun x1 -> 
@@ -60,24 +66,11 @@ let swap_and_sum' () =
   bind_elab (hwrite' 1 x0) (fun () ->
   return_elab (U32.v x0 + U32.v x1)))))
 
-val lswap_and_sum : unit -> lcomp_wp2 int sum_wp (reif sum_wp hswap_and_sum)
+val lswap_and_sum : unit -> lcomp_wp2 int sum_wp_full (reif sum_wp_full hswap_and_sum)
 let lswap_and_sum () =  
-  (* monotonicity *)
-  let mr1 = read_wp_mon 0 in
-  let mr1 = read_wp_mon 1 in
-  
   lbind (lread 0) (fun x0 -> 
   lbind (lread 1) (fun x1 -> 
-
-  (* monotonicity *)  
-  let mw1 = write_wp_mon 0 x1 in
-  let mw1 = write_wp_mon 1 x0 in     
-
   lbind (lwrite 0 x1) (fun () ->
-
-  let mret (_ : unit) = return_wp_mon (U32.v x0 + U32.v x1) in
-  let p' = forall_intro mret in 
-  assert (forall (_:unit). monotonic (return_wp (U32.v x0 + U32.v x1)));
   lbind (lwrite 1 x0) (fun () ->
   lreturn (U32.v x0 + U32.v x1)))))
   
